examples/hello.v
@@ -1,0 +1,122 @@
+Require Import isla.base.
+Require Import isla.opsem.
+Require Import isla.automation.
+Require Import isla.adequacy.
+Require Import isla.examples.sys_regs.
+From isla.instructions Require Import adrp_x1 mov_x2_4096 add_x1_x1_0x690 mov_w0_72 movk_x2 strb_w0_x2 ldrb_w0_x1 cbnz_w0_1 cbnz_w0_2.
+
+(*
+C code:
+	char *string = "Hello, World!\n";
+	while(*string) {
+		*(volatile char *)0x101f1000 = *string;
+		string++;
+	}
+
+ASM:
+.LC0:
+        .string "Hello, World!\n"
+main:
+        adrp    x1, .LC0
+        mov     x2, 4096
+        add	    x1, x1, #0x690
+        mov     w0, 72
+        movk    x2, 0x101f, lsl 16
+.L2:
+        strb    w0, [x2]
+        ldrb    w0, [x1, 1]!
+        cbnz    w0, .L2
+*)
+
+Definition hello_world_string : list byte :=
+  [ [BV{8} 0x48]; [BV{8} 0x65]; [BV{8} 0x6c]; [BV{8} 0x6c];  [BV{8} 0x6f]; [BV{8} 0x2c]; [BV{8} 0x20]; [BV{8} 0x57];  [BV{8} 0x6f]; [BV{8} 0x72]; [BV{8} 0x6c]; [BV{8} 0x64]; [BV{8} 0x21]; [BV{8} 0x0a]; [BV{8} 0x00]].
+
+Definition hello_world_string_printed : list byte :=
+  take (length hello_world_string - 1) hello_world_string.
+
+Definition hello_spec_trace : list seq_label :=
+  ((λ b : byte, SWriteMem [BV{64} 0x101f1000] b) <$> hello_world_string_printed) ++
+  [SInstrTrap [BV{64} 0x0000000010300020]].
+
+Definition hello_loop_spec `{!islaG Σ} `{!threadG} : iProp Σ :=
+  ∃ (i : nat),
+  ⌜i + 1 < length hello_world_string⌝ ∗
+  reg_col sys_regs ∗
+  [BV{64} 0x0000000010300690] ↦ₘ∗ hello_world_string ∗
+  "R2" ↦ᵣ Val_Bits [BV{64} 0x101f1000] ∗
+  "R1" ↦ᵣ Val_Bits (bv_add_Z [BV{64} 0x0000000010300690] i) ∗
+  "R0" ↦ᵣ Val_Bits (bv_zero_extend 64 (hello_world_string !!! i)) ∗
+  spec_trace (((λ b : byte, SWriteMem [BV{64} 0x101f1000] b) <$> (drop i hello_world_string_printed)) ++ [SInstrTrap [BV{64} 0x0000000010300020]]) ∗
+  True
+.
+
+Arguments hello_loop_spec /.
+
+Lemma hello_loop `{!islaG Σ} `{!threadG} :
+  instr 0x0000000010300014 (Some [strb_w0_x2_trace]) -∗
+  instr 0x0000000010300018 (Some [ldrb_w0_x1_trace]) -∗
+  instr 0x000000001030001c (Some [cbnz_w0_1; cbnz_w0_2]) -∗
+  instr 0x0000000010300020 None -∗
+  □ instr_pre 0x0000000010300014 hello_loop_spec -∗
+  mmio_range [BV{64} 0x101f1000] 0x10 -∗
+  instr_body 0x0000000010300014 hello_loop_spec.
+Proof.
+  iStartProof.
+  Time repeat liAStep; liShow.
+  liInst Hevar (S i)%nat.
+  Time repeat liAStep; liShow.
+  liInst Hevar (S i)%nat.
+  Time repeat liAStep; liShow.
+
+  Unshelve. all: prepare_sidecond.
+  all: try bv_solve.
+  - erewrite drop_S => /=.
+    2: { apply: list_lookup_lookup_total_lt => /=. lia. }
+    normalize_and_simpl_goal => //=. { bv_solve. }
+    rewrite lookup_total_take /=; [|lia].
+    by bv_simplify.
+  - erewrite drop_S; csimpl.
+    2: { apply: list_lookup_lookup_total_lt => /=. lia. }
+    rewrite drop_ge => //=.
+    rename select (bv_extract 0 _ _ = _) into Heq.
+    bv_simplify_hyp Heq.
+    revert select (_ !! i = Some vmem). move: Heq. clear => ??.
+    by repeat (destruct i; simplify_eq/=).
+  - rename select (bv_extract 0 _ _ ≠ _) into Hneq.
+    bv_simplify_hyp Hneq.
+    revert select (_ !! i = Some vmem). move: Hneq. clear => ??.
+    by repeat (destruct i; simplify_eq/=).
+  - erewrite list_lookup_total_correct; [|done]. bv_solve.
+  - erewrite drop_S; csimpl.
+    2: { apply: list_lookup_lookup_total_lt => /=. lia. }
+    done.
+Time Qed.
+
+
+Lemma hello `{!islaG Σ} `{!threadG} :
+  instr 0x0000000010300000 (Some [adrp_x1_trace]) -∗
+  instr 0x0000000010300004 (Some [mov_x2_4096_trace]) -∗
+  instr 0x0000000010300008 (Some [add_x1_x1_0x690_trace]) -∗
+  instr 0x000000001030000c (Some [mov_w0_72_trace]) -∗
+  instr 0x0000000010300010 (Some [movk_x2_trace]) -∗
+  □ instr_pre 0x0000000010300014 hello_loop_spec -∗
+  instr_body 0x0000000010300000 (
+    reg_col sys_regs ∗
+    [BV{64} 0x0000000010300690] ↦ₘ∗ hello_world_string ∗
+    "_PC" ↦ᵣ Val_Bits [BV{64} 0x0000000010300000 - 0x4] ∗
+    "__PC_changed" ↦ᵣ Val_Bool false ∗
+    "R0" ↦ᵣ Val_Poison ∗
+    "R1" ↦ᵣ Val_Poison ∗
+    "R2" ↦ᵣ Val_Poison ∗
+    "R11" ↦ᵣ Val_Poison ∗
+    spec_trace hello_spec_trace ∗
+    True)
+    .
+Proof.
+  iStartProof.
+  Time repeat liAStep; liShow.
+  liInst Hevar 0%nat.
+  Time repeat liAStep; liShow.
+  Unshelve. all: prepare_sidecond.
+  all: bv_simplify; try done.
+Time Qed.
