instructions/strb_w0_x2.v
@@ -1,0 +1,94 @@
+From isla Require Import isla_lang.
+
+Definition strb_w0_x2_trace : trc := [
+  Smt (DeclareConst 6%Z (Ty_BitVec 1%N)) Mk_annot;
+  Smt (DeclareConst 28%Z (Ty_BitVec 1%N)) Mk_annot;
+  Smt (DeclareConst 29%Z (Ty_BitVec 64%N)) Mk_annot;
+  Smt (Assert (Binop (Eq) (Manyop (Bvmanyarith Bvand) [Val (Val_Symbolic 29%Z) Mk_annot; Val (Val_Bits [BV{64%N} 0xfff0000000000007%Z]) Mk_annot] Mk_annot) (Val (Val_Bits [BV{64%N} 0x0%Z]) Mk_annot) Mk_annot)) Mk_annot;
+(*  Cycle Mk_annot;*)
+(*  ReadReg "SEE" [] (Val_I (-1)%Z 128%Z) Mk_annot;*)
+(*  WriteReg "SEE" [] (Val_I 1349%Z 128%Z) Mk_annot;*)
+(*  WriteReg "__unconditional" [] (Val_Bool true) Mk_annot;*)
+(*  ReadReg "__v85_implemented" [] (Val_Bool false) Mk_annot;*)
+  ReadReg "R2" [] (Val_Symbolic 29%Z) Mk_annot;
+  Smt (DefineConst 89%Z (Manyop (Bvmanyarith Bvadd) [Val (Val_Symbolic 29%Z) Mk_annot; Val (Val_Bits [BV{64%N} 0x0%Z]) Mk_annot] Mk_annot)) Mk_annot;
+  Smt (DeclareConst 90%Z (Ty_BitVec 64%N)) Mk_annot;
+  ReadReg "R0" [] (Val_Symbolic 90%Z) Mk_annot;
+  Smt (DefineConst 91%Z (Unop (Extract 7%N 0%N) (Val (Val_Symbolic 90%Z) Mk_annot) Mk_annot)) Mk_annot;
+  ReadReg "PSTATE" [Field "EL"] (Val_Struct [("EL", Val_Bits [BV{2%N} 0x2%Z])]) Mk_annot;
+(*  ReadReg "__v84_implemented" [] (Val_Bool false) Mk_annot;*)
+  ReadReg "PSTATE" [Field "nRW"] (Val_Struct [("nRW", Val_Symbolic 28%Z)]) Mk_annot;
+  Smt (DefineConst 93%Z (Binop (Eq) (Val (Val_Symbolic 28%Z) Mk_annot) (Val (Val_Bits [BV{1%N} 0x1%Z]) Mk_annot) Mk_annot)) Mk_annot;
+  ReadReg "CFG_ID_AA64PFR0_EL1_EL0" [] (Val_Bits [BV{4%N} 0x1%Z]) Mk_annot;
+  ReadReg "CFG_ID_AA64PFR0_EL1_EL1" [] (Val_Bits [BV{4%N} 0x1%Z]) Mk_annot;
+  ReadReg "CFG_ID_AA64PFR0_EL1_EL2" [] (Val_Bits [BV{4%N} 0x1%Z]) Mk_annot;
+  ReadReg "CFG_ID_AA64PFR0_EL1_EL3" [] (Val_Bits [BV{4%N} 0x1%Z]) Mk_annot;
+  Smt (Assert (Unop (Not) (Val (Val_Symbolic 93%Z) Mk_annot) Mk_annot)) Mk_annot;
+(*  ReadReg "__highest_el_aarch32" [] (Val_Bool false) Mk_annot;*)
+  Smt (Assert (Unop (Not) (Val (Val_Symbolic 93%Z) Mk_annot) Mk_annot)) Mk_annot;
+  ReadReg "SCTLR_EL2" [] (Val_Bits [BV{64%N} 0x4000002%Z]) Mk_annot;
+  Smt (DefineConst 98%Z (Binop (Eq) (Val (Val_Symbolic 89%Z) Mk_annot) (Manyop (Bvmanyarith Bvand) [Val (Val_Symbolic 89%Z) Mk_annot; Val (Val_Bits [BV{64%N} 0xffffffffffffffff%Z]) Mk_annot] Mk_annot) Mk_annot)) Mk_annot;
+  Smt (Assert (Unop (Not) (Unop (Not) (Val (Val_Symbolic 98%Z) Mk_annot) Mk_annot) Mk_annot)) Mk_annot;
+  Smt (Assert (Unop (Not) (Unop (Not) (Val (Val_Symbolic 98%Z) Mk_annot) Mk_annot) Mk_annot)) Mk_annot;
+  Smt (Assert (Binop (Eq) (Val (Val_Symbolic 89%Z) Mk_annot) (Manyop (Bvmanyarith Bvand) [Val (Val_Symbolic 89%Z) Mk_annot; Val (Val_Bits [BV{64%N} 0xffffffffffffffff%Z]) Mk_annot] Mk_annot) Mk_annot)) Mk_annot;
+  Smt (DefineConst 293%Z (Binop (Eq) (Val (Val_Symbolic 28%Z) Mk_annot) (Val (Val_Bits [BV{1%N} 0x1%Z]) Mk_annot) Mk_annot)) Mk_annot;
+  Smt (Assert (Unop (Not) (Val (Val_Symbolic 293%Z) Mk_annot) Mk_annot)) Mk_annot;
+  Smt (Assert (Unop (Not) (Val (Val_Symbolic 293%Z) Mk_annot) Mk_annot)) Mk_annot;
+  Smt (DefineConst 296%Z (Binop (Eq) (Val (Val_Symbolic 28%Z) Mk_annot) (Val (Val_Bits [BV{1%N} 0x1%Z]) Mk_annot) Mk_annot)) Mk_annot;
+  Smt (Assert (Unop (Not) (Val (Val_Symbolic 296%Z) Mk_annot) Mk_annot)) Mk_annot;
+  Smt (Assert (Unop (Not) (Val (Val_Symbolic 296%Z) Mk_annot) Mk_annot)) Mk_annot;
+  ReadReg "SCR_EL3" [] (Val_Bits [BV{32%N} 0x0%Z]) Mk_annot;
+(*  ReadReg "__v81_implemented" [] (Val_Bool true) Mk_annot;*)
+  ReadReg "TCR_EL2" [] (Val_Bits [BV{64%N} 0x0%Z]) Mk_annot;
+(*  ReadReg "__v83_implemented" [] (Val_Bool false) Mk_annot;*)
+  Smt (Assert (Unop (Not) (Unop (Not) (Binop (Eq) (Unop (Extract 63%N 52%N) (Val (Val_Symbolic 89%Z) Mk_annot) Mk_annot) (Val (Val_Bits [BV{12%N} 0x0%Z]) Mk_annot) Mk_annot) Mk_annot) Mk_annot)) Mk_annot;
+  Smt (DefineConst 908%Z (Binop (Eq) (Val (Val_Symbolic 28%Z) Mk_annot) (Val (Val_Bits [BV{1%N} 0x1%Z]) Mk_annot) Mk_annot)) Mk_annot;
+  Smt (Assert (Unop (Not) (Val (Val_Symbolic 908%Z) Mk_annot) Mk_annot)) Mk_annot;
+  Smt (Assert (Unop (Not) (Val (Val_Symbolic 908%Z) Mk_annot) Mk_annot)) Mk_annot;
+  Smt (DefineConst 911%Z (Binop (Eq) (Val (Val_Symbolic 28%Z) Mk_annot) (Val (Val_Bits [BV{1%N} 0x1%Z]) Mk_annot) Mk_annot)) Mk_annot;
+  Smt (Assert (Unop (Not) (Val (Val_Symbolic 911%Z) Mk_annot) Mk_annot)) Mk_annot;
+  Smt (Assert (Unop (Not) (Val (Val_Symbolic 911%Z) Mk_annot) Mk_annot)) Mk_annot;
+  Smt (DefineConst 940%Z (Binop (Eq) (Val (Val_Symbolic 28%Z) Mk_annot) (Val (Val_Bits [BV{1%N} 0x1%Z]) Mk_annot) Mk_annot)) Mk_annot;
+  Smt (Assert (Unop (Not) (Val (Val_Symbolic 940%Z) Mk_annot) Mk_annot)) Mk_annot;
+  Smt (Assert (Unop (Not) (Val (Val_Symbolic 940%Z) Mk_annot) Mk_annot)) Mk_annot;
+  Smt (DefineConst 943%Z (Binop (Eq) (Val (Val_Symbolic 28%Z) Mk_annot) (Val (Val_Bits [BV{1%N} 0x1%Z]) Mk_annot) Mk_annot)) Mk_annot;
+  Smt (Assert (Unop (Not) (Val (Val_Symbolic 943%Z) Mk_annot) Mk_annot)) Mk_annot;
+  Smt (Assert (Unop (Not) (Val (Val_Symbolic 943%Z) Mk_annot) Mk_annot)) Mk_annot;
+  Smt (DefineConst 982%Z (Binop (Eq) (Val (Val_Symbolic 28%Z) Mk_annot) (Val (Val_Bits [BV{1%N} 0x1%Z]) Mk_annot) Mk_annot)) Mk_annot;
+  Smt (Assert (Unop (Not) (Val (Val_Symbolic 982%Z) Mk_annot) Mk_annot)) Mk_annot;
+  Smt (Assert (Unop (Not) (Val (Val_Symbolic 982%Z) Mk_annot) Mk_annot)) Mk_annot;
+  Smt (Assert (Unop (Not) (Unop (Not) (Val (Val_Symbolic 98%Z) Mk_annot) Mk_annot) Mk_annot)) Mk_annot;
+  Smt (DefineConst 1190%Z (Binop (Eq) (Val (Val_Symbolic 28%Z) Mk_annot) (Val (Val_Bits [BV{1%N} 0x1%Z]) Mk_annot) Mk_annot)) Mk_annot;
+  Smt (Assert (Unop (Not) (Val (Val_Symbolic 1190%Z) Mk_annot) Mk_annot)) Mk_annot;
+  Smt (Assert (Unop (Not) (Val (Val_Symbolic 1190%Z) Mk_annot) Mk_annot)) Mk_annot;
+  Smt (DefineConst 1193%Z (Binop (Eq) (Val (Val_Symbolic 28%Z) Mk_annot) (Val (Val_Bits [BV{1%N} 0x1%Z]) Mk_annot) Mk_annot)) Mk_annot;
+  Smt (Assert (Unop (Not) (Val (Val_Symbolic 1193%Z) Mk_annot) Mk_annot)) Mk_annot;
+  Smt (Assert (Unop (Not) (Val (Val_Symbolic 1193%Z) Mk_annot) Mk_annot)) Mk_annot;
+  Smt (DefineConst 1232%Z (Binop (Eq) (Val (Val_Symbolic 28%Z) Mk_annot) (Val (Val_Bits [BV{1%N} 0x1%Z]) Mk_annot) Mk_annot)) Mk_annot;
+  Smt (Assert (Unop (Not) (Val (Val_Symbolic 1232%Z) Mk_annot) Mk_annot)) Mk_annot;
+  Smt (Assert (Unop (Not) (Val (Val_Symbolic 1232%Z) Mk_annot) Mk_annot)) Mk_annot;
+  Smt (DefineConst 1235%Z (Binop (Eq) (Val (Val_Symbolic 28%Z) Mk_annot) (Val (Val_Bits [BV{1%N} 0x1%Z]) Mk_annot) Mk_annot)) Mk_annot;
+  Smt (Assert (Unop (Not) (Val (Val_Symbolic 1235%Z) Mk_annot) Mk_annot)) Mk_annot;
+  Smt (Assert (Unop (Not) (Val (Val_Symbolic 1235%Z) Mk_annot) Mk_annot)) Mk_annot;
+  ReadReg "PSTATE" [Field "D"] (Val_Struct [("D", Val_Symbolic 6%Z)]) Mk_annot;
+  ReadReg "OSLSR_EL1" [] (Val_Bits [BV{32%N} 0x0%Z]) Mk_annot;
+  ReadReg "OSDLR_EL1" [] (Val_Bits [BV{32%N} 0x0%Z]) Mk_annot;
+  ReadReg "EDSCR" [] (Val_Bits [BV{32%N} 0x0%Z]) Mk_annot;
+  Smt (DeclareConst 1248%Z (Ty_BitVec 64%N)) Mk_annot;
+  ReadReg "MPIDR_EL1" [] (Val_Symbolic 1248%Z) Mk_annot;
+  Smt (DefineConst 1279%Z (Binop (Eq) (Val (Val_Symbolic 28%Z) Mk_annot) (Val (Val_Bits [BV{1%N} 0x1%Z]) Mk_annot) Mk_annot)) Mk_annot;
+  Smt (Assert (Unop (Not) (Val (Val_Symbolic 1279%Z) Mk_annot) Mk_annot)) Mk_annot;
+  Smt (Assert (Unop (Not) (Val (Val_Symbolic 1279%Z) Mk_annot) Mk_annot)) Mk_annot;
+  Smt (DefineConst 1282%Z (Binop (Eq) (Val (Val_Symbolic 28%Z) Mk_annot) (Val (Val_Bits [BV{1%N} 0x1%Z]) Mk_annot) Mk_annot)) Mk_annot;
+  Smt (Assert (Unop (Not) (Val (Val_Symbolic 1282%Z) Mk_annot) Mk_annot)) Mk_annot;
+  Smt (Assert (Unop (Not) (Val (Val_Symbolic 1282%Z) Mk_annot) Mk_annot)) Mk_annot;
+(*  ReadReg "__v82_implemented" [] (Val_Bool false) Mk_annot;*)
+(*  ReadReg "__trickbox_enabled" [] (Val_Bool false) Mk_annot;*)
+(*  ReadReg "__CNTControlBase" [] (Val_Bits [BV{52%N} 0x0%Z]) Mk_annot;*)
+  Smt (DeclareConst 1322%Z (Ty_BitVec 56%N)) Mk_annot;
+(*  ReadReg "__defaultRAM" [] (Val_Symbolic 1322%Z) Mk_annot;*)
+(*  ReadReg "__isla_monomorphize_writes" [] (Val_Bool false) Mk_annot;*)
+  Smt (DefineConst 1335%Z (Unop (ZeroExtend 8%N) (Manyop Concat [Val (Val_Bits [BV{4%N} 0x0%Z]) Mk_annot; Unop (Extract 51%N 0%N) (Val (Val_Symbolic 89%Z) Mk_annot) Mk_annot] Mk_annot) Mk_annot)) Mk_annot;
+  Smt (DeclareConst 1336%Z Ty_Bool) Mk_annot;
+  WriteMem (Val_Symbolic 1336%Z) (Val_Enum ((Mk_enum_id 6%nat), Mk_enum_ctor 0%nat)) (Val_Symbolic 1335%Z) (Val_Symbolic 91%Z) 1%N None Mk_annot
+].
